removing typeclasses

Simulator/CoqSim/Eval.v
@@ -5,32 +5,24 @@ Require Import Kami.AllNotations.
 
 Require Import Kami.Simulator.CoqSim.Misc.
 Require Import Kami.Simulator.CoqSim.TransparentProofs.
-Require Import Kami.Simulator.CoqSim.SimTypes.
 Require Import Kami.Simulator.CoqSim.HaskellTypes.
+Import Kami.Simulator.CoqSim.HaskellTypes.Notations.
 
 Section Eval.
-
-Variable Word : nat -> Type.
-Variable Vec : nat -> Type -> Type.
-Variable M : Type -> Type.
-
-Context `{IsWord Word}.
-Context `{IsVector Vec}.
-Context `{IOMonad Word Vec M}.
 
 Fixpoint eval_Kind(k : Kind) : Type :=
   match k with
   | Bool => bool
-  | Bit n => Word n
+  | Bit n => BV n
   | Struct n ks fs => Tuple (fun i => eval_Kind (ks i))
-  | Array n k' => Vec n (eval_Kind k')
+  | Array n k' => Vector n (eval_Kind k')
   end.
 
-Definition print_BF(bf : BitFormat){n} : Word n -> string :=
+Definition print_BF(bf : BitFormat){n} : BV n -> string :=
   match bf with
-  | Binary => print_word_bin
-  | Decimal => print_word_dec
-  | Hex => print_word_hex
+  | Binary => print_bv_bin
+  | Decimal => print_bv_dec
+  | Hex => print_bv_hex
   end.
 
 Fixpoint print_Kind(k : Kind)(ff : FullFormat k) : eval_Kind k -> string :=
@@ -38,15 +30,15 @@ Fixpoint print_Kind(k : Kind)(ff : FullFormat k) : eval_Kind k -> string :=
   | FBool n _ => fun x => space_pad n (if x then "1" else "0")
   | FBit n m bf => fun x => (*zero_pad m*) (print_BF bf x)
   | FStruct n fk fs ffs => fun x => ("{ " ++ String.concat "; " (v_to_list (vmap (fun '(str1,str2) => str1 ++ ":" ++ str2) (add_strings fs (tup_to_vec _ (fun i => print_Kind (ffs i)) x)))) ++ "; }")%string
-  | FArray n k' ff' => fun x => ("[" ++ String.concat "; " (List.map (fun i => nat_decimal_string (f2n i) ++ "=" ++ print_Kind ff' (index i x)) (getFins n)) ++ "; ]")%string
+  | FArray n k' ff' => fun x => ("[" ++ String.concat "; " (List.map (fun i => nat_decimal_string (f2n i) ++ "=" ++ print_Kind ff' (vector_index i x)) (getFins n)) ++ "; ]")%string
   end.
 
 Fixpoint Kind_eq{k} : eval_Kind k -> eval_Kind k -> bool :=
   match k return eval_Kind k -> eval_Kind k -> bool with
   | Bool => Bool.eqb
-  | Bit n => weqb
+  | Bit n => bv_eq
   | Struct n ks fs => TupEq (fun i => eval_Kind (ks i)) (fun i => @Kind_eq (ks i))
-  | Array n k' => vec_eq (@Kind_eq k')
+  | Array n k' => vector_eq (@Kind_eq k')
   end.
 
 Definition eval_FK(k : FullKind) :=
@@ -55,14 +47,12 @@ Definition eval_FK(k : FullKind) :=
   | NativeKind t _ => t
   end.
 
-Notation "'do' x <- y ; cont" := (bind y (fun x => cont)) (at level 20).
-
 Fixpoint default_val(k : Kind) : eval_Kind k :=
   match k return eval_Kind k with
   | Bool => false
-  | Bit n => nat_to_word 0
+  | Bit n => nat_to_bv 0
   | Struct n ks fs => mkTup (fun i => eval_Kind (ks i)) (fun i => default_val (ks i))
-  | Array n k' => make_vec (fun _ => default_val k')
+  | Array n k' => make_vector (fun _ => default_val k')
   end.
 
 Definition default_val_FK(k : FullKind) : eval_FK k :=
@@ -71,7 +61,7 @@ Definition default_val_FK(k : FullKind) : eval_FK k :=
   | NativeKind T t => t
   end.
 
-Fixpoint rand_tuple{n} : forall ts : Fin.t n -> Type, (forall i, M (ts i)) -> M (Tuple ts) :=
+Fixpoint rand_tuple{n} : forall ts : Fin.t n -> Type, (forall i, IO (ts i)) -> IO (Tuple ts) :=
   match n with
   | 0 => fun _ _ => ret tt
   | S m => fun ts mxs => (
@@ -81,15 +71,15 @@ Fixpoint rand_tuple{n} : forall ts : Fin.t n -> Type, (forall i, M (ts i)) -> M 
       )
   end.
 
-Fixpoint rand_val(k : Kind) : M (eval_Kind k) :=
-  match k return M (eval_Kind k) with
+Fixpoint rand_val(k : Kind) : IO (eval_Kind k) :=
+  match k return IO (eval_Kind k) with
   | Bool => rand_bool
-  | Bit n => rand_word n
+  | Bit n => rand_bv n
   | Struct n ks fs => rand_tuple (fun i => eval_Kind (ks i)) (fun i => rand_val (ks i))
-  | Array n k' => rand_vec (rand_val k')
+  | Array n k' => rand_vector (rand_val k')
   end.
 
-Fixpoint rand_val_FK(k : FullKind) : M (eval_FK k) :=
+Fixpoint rand_val_FK(k : FullKind) : IO (eval_FK k) :=
   match k with
   | SyntaxKind k' => rand_val k'
   | NativeKind k' c => ret c
@@ -107,47 +97,47 @@ Definition eval_CABool(op : CABoolOp) : list bool -> bool :=
   | Xor => fun xs => fold_left xorb xs false
   end.
 
-Definition eval_UniBit{m n}(op : UniBitOp m n) : Word m -> Word n :=
+Definition eval_UniBit{m n}(op : UniBitOp m n) : BV m -> BV n :=
   match op with
-  | Inv n => inv
-  | TruncLsb lsb msb => trunc_lsb
-  | TruncMsb lsb msb => trunc_msb
-  | UAnd n => uand
-  | UOr n => uor
-  | UXor n => uxor
+  | Inv n => bv_inv
+  | TruncLsb lsb msb => bv_trunc_lsb
+  | TruncMsb lsb msb => bv_trunc_msb
+  | UAnd n => bv_uand
+  | UOr n => bv_uor
+  | UXor n => bv_uxor
   end.
 
-Definition eval_BinBit{m n p}(op : BinBitOp m n p) : Word m -> Word n -> Word p :=
+Definition eval_BinBit{m n p}(op : BinBitOp m n p) : BV m -> BV n -> BV p :=
   match op with
-  | Sub n => sub
-  | Div n => div
-  | Rem n => rem
-  | Sll n m => sll
-  | Srl n m => srl
-  | Sra n m => sra
-  | Concat msb lsb => concat
+  | Sub n => bv_sub
+  | Div n => bv_div
+  | Rem n => bv_rem
+  | Sll n m => bv_sll
+  | Srl n m => bv_srl
+  | Sra n m => bv_sra
+  | Concat msb lsb => bv_concat
   end.
 
-Definition eval_CABit{n}(op : CABitOp) : list (Word n) -> Word n :=
+Definition eval_CABit{n}(op : CABitOp) : list (BV n) -> BV n :=
   match op with
-  | Add => add
-  | Mul => mul
-  | Band => band
-  | Bor => bor
-  | Bxor => bxor
+  | Add => bv_add
+  | Mul => bv_mul
+  | Band => bv_band
+  | Bor => bv_bor
+  | Bxor => bv_bxor
   end.
 
-Definition eval_BinBitBool{m n}(op : BinBitBoolOp m n) : Word m -> Word n -> bool :=
+Definition eval_BinBitBool{m n}(op : BinBitBoolOp m n) : BV m -> BV n -> bool :=
   match op with
-  | LessThan n => wltb
+  | LessThan n => bv_lt
   end.
 
 Fixpoint eval_ConstT{k}(e : ConstT k) : eval_Kind k :=
   match e with
   | ConstBool b => b
-  | ConstBit n w => nat_to_word (wordToNat w)
+  | ConstBit n w => nat_to_bv (wordToNat w)
   | ConstStruct n ks ss es => mkTup (fun i => eval_Kind (ks i)) (fun i => eval_ConstT (es i))
-  | ConstArray n k' es => make_vec (fun i => eval_ConstT (es i))
+  | ConstArray n k' es => make_vector (fun i => eval_ConstT (es i))
   end.
 
 Definition eval_ConstFullT{k} (e : ConstFullT k) : eval_FK k :=
@@ -170,20 +160,20 @@ Fixpoint eval_Expr{k}(e : Expr eval_Kind k) : eval_FK k :=
   | Eq _ e1 e2 => Kind_eq (eval_Expr e1) (eval_Expr e2)
   | ReadStruct n ks ss e i => tup_index i _ (eval_Expr e)
   | BuildStruct n ks ss es => mkTup _ (fun i => eval_Expr (es i))
-  | ReadArray n m k v i => match lt_dec (word_to_nat (eval_Expr i)) n with
-                           | left pf => index (Fin.of_nat_lt pf) (eval_Expr v)
+  | ReadArray n m k v i => match lt_dec (bv_to_nat (eval_Expr i)) n with
+                           | left pf => vector_index (Fin.of_nat_lt pf) (eval_Expr v)
                            | right _ => eval_ConstT (getDefaultConst k)
                            end
-  | ReadArrayConst n k v i => index i (eval_Expr v)
-  | BuildArray n k v => make_vec (fun i => eval_Expr (v i))
+  | ReadArrayConst n k v i => vector_index i (eval_Expr v)
+  | BuildArray n k v => make_vector (fun i => eval_Expr (v i))
   end.
 
-(* Fixpoint val_unpack'(k : Kind) : Word (size k) -> eval_Kind k.
+(* Fixpoint val_unpack'(k : Kind) : BV (size k) -> eval_Kind k.
 Proof.
   induction k; simpl; intro e.
   (* Bool *)
   - exact (weqb e (nat_to_word 1)).
-  (* Word *)
+  (* BV *)
   - exact e.
   (* Tup *)
   - admit.
@@ -191,17 +181,17 @@ Proof.
  *)
 
 
-Definition val_unpack(k : Kind) : Word (size k) -> eval_Kind k :=
-  fun w => eval_Expr (unpack _ (Const _ (ConstBit (natToWord _ (word_to_nat w))))).
+Definition val_unpack(k : Kind) : BV (size k) -> eval_Kind k :=
+  fun w => eval_Expr (unpack _ (Const _ (ConstBit (natToWord _ (bv_to_nat w))))).
 
-Definition eval_SysT(s : SysT eval_Kind) : M unit :=
+Definition eval_SysT(s : SysT eval_Kind) : IO unit :=
   match s with
   | DispString s => print s
   | DispExpr k e ff => print (print_Kind ff (eval_Expr e))
   | Finish => exit
   end.
 
-Fixpoint eval_list_SysT(xs : list (SysT eval_Kind)) : M unit :=
+Fixpoint eval_list_SysT(xs : list (SysT eval_Kind)) : IO unit :=
   match xs with
   | [] => ret tt
   | s::ys => (
