Simulator/CoqSim/Simulator.v
@@ -3,33 +3,16 @@ Require Import Streams.
 
 Require Import Kami.Simulator.CoqSim.Misc.
 Require Import Kami.Simulator.CoqSim.TransparentProofs.
-Require Import Kami.Simulator.CoqSim.SimTypes.
 Require Import Kami.Simulator.CoqSim.HaskellTypes.
 Require Import Kami.Simulator.CoqSim.RegisterFile.
 Require Import Kami.Simulator.CoqSim.Eval.
 
 Require Import Kami.AllNotations.
+Import Kami.Simulator.CoqSim.HaskellTypes.Notations.
+
 Section EvalAction.
 
-Variable Word : nat -> Type.
-Variable Vec : nat -> Type -> Type.
-Variable Map : Type -> Type.
-Variable M : Type -> Type.
-Variable Arr : Type -> Type.
-
-Context `{IsWord Word}.
-Context `{IsVector Vec}.
-Context `{StringMap Map}.
-Context `{IOMonad Word Vec M}.
-Context `{IsArray Word Vec M Arr}.
-
-Notation "'do' x <- y ; cont" := (bind y (fun x => cont)) (at level 20).
-
-Definition eval_K := eval_Kind Word Vec.
-
-Definition eval_E := @eval_Expr Word Vec _ _.
-
-Definition SimReg := (string * {x : _ & fullType eval_K x})%type.
+Definition SimReg := (string * {x : _ & fullType eval_Kind x})%type.
 Definition SimRegs := list SimReg.
 
 Section Regs.
@@ -62,12 +45,12 @@ Record Update := {
   reg_name : string;
   kind : FullKind;
   init_val : RegInitValT kind;
-  new_val : fullType eval_K kind;
+  new_val : fullType eval_Kind kind;
   lookup_match : lookup String.eqb reg_name init_regs = Some (existT _ kind init_val)
   }.
 
 Definition Updates := list Update.
-Definition FileUpdates := list (@FileUpd Vec Word).
+Definition FileUpdates := list FileUpd.
 
 Fixpoint mkProd(ts : list Type) : Type :=
   match ts with
@@ -76,12 +59,12 @@ Fixpoint mkProd(ts : list Type) : Type :=
   end.
 
 Class Environment E := {
-  envPre  : E -> FileState (V := Vec) (W := Word) (M := Map) (Arr := Arr) -> SimRegs -> string -> M E;
-  envPost : E -> FileState (V := Vec) (W := Word) (M := Map) (Arr := Arr) -> SimRegs -> string -> M E
+  envPre  : E -> FileState -> SimRegs -> string -> IO E;
+  envPost : E -> FileState -> SimRegs -> string -> IO E
   }.
 
 Definition meth_sig{E}`{Environment E}(sig : Signature) : Type :=
-  eval_K (fst sig) -> FileState (V := Vec) (W := Word) (M := Map) (Arr := Arr) -> SimRegs -> E -> M (E * (eval_K (snd sig))).
+  eval_Kind (fst sig) -> FileState -> SimRegs -> E -> IO (E * (eval_Kind (snd sig))).
 
 Definition dec_sig{E}`{Environment E}(dec : string * Signature) : Type :=
   meth_sig (snd dec).
@@ -97,16 +80,16 @@ Fixpoint return_meth{E}`{Environment E}(meth : string)(sig : Signature)(meths : 
 Proof.
   assert (sig = snd dec).
   rewrite <- pf; auto.
-  rewrite H12.
+  rewrite H0.
   exact (fst fs).
 Defined.
 
-Definition reg_not_found{X} : string -> M X :=
+Definition reg_not_found{X} : string -> IO X :=
   fun reg => error ("register " ++ reg ++ " not found.").
 
-Fixpoint eval_ActionT{k}{E}`{Environment E}(env : E)(state : @FileState Vec Word Map Arr)(meths : list (string * Signature))(updates : Updates)(fupdates : FileUpdates)(a : ActionT eval_K k)(a_wf : WfActionT_new init_regs a)(fs : mkProd (List.map dec_sig meths)){struct a} : M (Updates * FileUpdates * eval_K k).
+Fixpoint eval_ActionT{k}{E}`{Environment E}(env : E)(state : FileState)(meths : list (string * Signature))(updates : Updates)(fupdates : FileUpdates)(a : ActionT eval_Kind k)(a_wf : WfActionT_new init_regs a)(fs : mkProd (List.map dec_sig meths)){struct a} : IO (Updates * FileUpdates * eval_Kind k).
   refine (match a return WfActionT_new init_regs a -> _ with
-  | MCall meth s e cont => fun pf => io_do x <- rf_methcall state meth (existT _ (fst s) (eval_E e));
+  | MCall meth s e cont => fun pf => do x <- rf_methcall state meth (existT _ (fst s) (eval_Expr e));
        match x with
       | Some (o, existT k v) => match Kind_dec k (snd s) with
                                 | left _ => _
@@ -167,8 +150,8 @@ Proof.
            inversion G; auto.
         ** destruct pf.
            clear G.
-           rewrite <- H12, <- H13 in f.
-           exact (eval_ActionT _ _ _ env state meths updates fupdates (cont f) (H14 _) fs).
+           rewrite <- H0, <- H1 in f.
+           exact (eval_ActionT _ _ _ env state meths updates fupdates (cont f) (H2 _) fs).
       * destruct pf.
    + exact (reg_not_found r).
   (* WriteReg *)
@@ -215,8 +198,8 @@ Fixpoint curry(X : Type)(ts : list Type) : (mkProd ts -> X) -> curried X ts :=
   | T::ts' => fun f t => curry ts' (fun xs => f (t,xs))
   end.
 
-Definition eval_RuleT{E}`{Environment E}(env : E)(state : FileState)(meths : list (string * Signature))(r : RuleT)(r_wf : WfActionT_new init_regs (snd r eval_K))(fs : mkProd (List.map dec_sig meths)) : M (Updates * FileUpdates * eval_K Void) :=
-  eval_ActionT env state meths [] [] ((snd r) eval_K) r_wf fs.
+Definition eval_RuleT{E}`{Environment E}(env : E)(state : FileState)(meths : list (string * Signature))(r : RuleT)(r_wf : WfActionT_new init_regs (snd r eval_Kind))(fs : mkProd (List.map dec_sig meths)) : IO (Updates * FileUpdates * eval_Kind Void) :=
+  eval_ActionT env state meths [] [] ((snd r) eval_Kind) r_wf fs.
 
 Fixpoint do_single_update(upd : Update)(regs : SimRegs) : SimRegs :=
   match regs with
@@ -234,7 +217,7 @@ Section Regs2.
 Lemma update_hit : forall init_regs regs k v (upd : Update init_regs), lookup String.eqb (reg_name upd) regs = Some (existT _ k v) -> lookup String.eqb (reg_name upd) (do_single_update upd regs) = Some (existT _ (kind upd) (new_val upd)).
 Proof.
   induction regs; intros.
-  - discriminate H11.
+  - discriminate H.
   - simpl do_single_update.
     destruct a.
     destruct String.eqb eqn:G.
@@ -244,9 +227,9 @@ Proof.
     + rewrite lookup_cons.
       rewrite G.
       eapply IHregs.
-      rewrite lookup_cons in H11.
-      rewrite G in H11.
-      exact H11.
+      rewrite lookup_cons in H.
+      rewrite G in H.
+      exact H.
 Qed.
 
 Lemma update_miss : forall r init_regs regs (upd : Update init_regs), r <> reg_name upd -> lookup String.eqb r (do_single_update upd regs) = lookup String.eqb r regs.
@@ -258,9 +241,9 @@ Proof.
     destruct String.eqb eqn:G.
     + repeat rewrite lookup_cons.
       rewrite String.eqb_eq in G.
-      rewrite G in H11.
-      rewrite <- String.eqb_neq in H11.
-      rewrite H11.
+      rewrite G in H.
+      rewrite <- String.eqb_neq in H.
+      rewrite H.
       auto.
     + repeat rewrite lookup_cons.
       destruct (r =? s).
@@ -268,24 +251,24 @@ Proof.
       * apply IHregs; auto.
 Qed.
 
-Lemma lookup_update : forall init_regs regs k x (upd : Update init_regs) r, lookup String.eqb r (do_single_update upd regs) = Some (existT (fun x : FullKind => fullType eval_K x) k x) -> exists k' y, lookup String.eqb r regs = Some (existT _ k' y).
+Lemma lookup_update : forall init_regs regs k x (upd : Update init_regs) r, lookup String.eqb r (do_single_update upd regs) = Some (existT (fun x : FullKind => fullType eval_Kind x) k x) -> exists k' y, lookup String.eqb r regs = Some (existT _ k' y).
 Proof.
   induction regs; intros.
-  - discriminate H11.
-  - simpl do_single_update in H11.
+  - discriminate H.
+  - simpl do_single_update in H.
     destruct a.
     destruct (reg_name upd =? s).
-    + rewrite lookup_cons in H11.
+    + rewrite lookup_cons in H.
       rewrite lookup_cons.
       destruct (r =? s).
       * destruct s0; repeat eexists; reflexivity.
-      * repeat eexists; exact H11.
-    + rewrite lookup_cons in H11.
+      * repeat eexists; exact H.
+    + rewrite lookup_cons in H.
       rewrite lookup_cons.
       destruct (r =? s).
       * destruct s0; repeat eexists; reflexivity.
       * eapply IHregs.
-        exact H11.
+        exact H.
 Qed.
 
 Lemma update_consistent : forall (curr_regs : SimRegs)(init_regs : list RegInitT)(upd : Update init_regs),
@@ -296,46 +279,46 @@ Proof.
   - destruct (String.eqb r (reg_name upd)) eqn:G.
     + rewrite String.eqb_eq in G.
       rewrite G.
-      destruct (kc_init_sim kc _ H11).
+      destruct (kc_init_sim kc _ H).
       erewrite update_hit.
       * pose (lookup_match upd) as lk.
         rewrite <- G in lk.
-        rewrite H11 in lk.
+        rewrite H in lk.
         inversion lk.
-        rewrite H14 in *.
+        rewrite H2 in *.
         eexists; auto.
       * rewrite <- G.
-        destruct (kc_init_sim kc _ H11).
-        exact H12.
+        destruct (kc_init_sim kc _ H).
+        exact H0.
     + rewrite String.eqb_neq in G.
       erewrite update_miss; auto.
       apply kc.
-      eexists; exact H11.
+      eexists; exact H.
   - destruct (String.eqb r (reg_name upd)) eqn:G.
     + rewrite String.eqb_eq in G.
-      rewrite G in H11.
-      destruct (lookup_update _ _ _ H11) as [k' [y Hy]].
-      erewrite update_hit in H11.
+      rewrite G in H.
+      destruct (lookup_update _ _ _ H) as [k' [y Hy]].
+      erewrite update_hit in H.
       * pose (lookup_match upd) as lk.
         rewrite G.
-        inversion H11.
+        inversion H.
         eexists; exact lk.
       * exact Hy.
     + rewrite String.eqb_neq in G.
-      erewrite update_miss in H11; auto.
-      destruct (kc_sim_init kc _ H11).
-      eexists; exact H12.
+      erewrite update_miss in H; auto.
+      destruct (kc_sim_init kc _ H).
+      eexists; exact H0.
 Qed.
 
 Lemma updates_consistent : forall (init_regs : list RegInitT)(curr_regs : SimRegs)(upds : list (Update init_regs)),
   kind_consistent init_regs curr_regs -> kind_consistent init_regs (do_updates upds curr_regs).
 Proof.
   induction upds; intro.
-  - exact H11.
+  - exact H.
   - apply update_consistent; auto.
 Qed.
 
-Fixpoint eval_Rules{E}`{Environment E}(env : E)(state : FileState (V := Vec) (W := Word) (M := Map) (Arr := Arr))(numRules : nat)(meths : list (string * Signature))(init_regs : list (string * {x : FullKind & RegInitValT x}))(curr_regs : SimRegs)(kc_curr : kind_consistent init_regs curr_regs)(rules : Stream {r : RuleT & WfActionT_new init_regs (snd r eval_K)}){struct numRules} : mkProd (List.map dec_sig meths) -> M unit. refine
+Fixpoint eval_Rules{E}`{Environment E}(env : E)(state : FileState)(numRules : nat)(meths : list (string * Signature))(init_regs : list (string * {x : FullKind & RegInitValT x}))(curr_regs : SimRegs)(kc_curr : kind_consistent init_regs curr_regs)(rules : Stream {r : RuleT & WfActionT_new init_regs (snd r eval_Kind)}){struct numRules} : mkProd (List.map dec_sig meths) -> IO unit. refine
   match numRules with
   | 0 => fun fs => error "TIMEOUT"
   | S numRules' => fun fs => match rules with
@@ -371,8 +354,8 @@ Proof.
   intros.
   induction rules.
   - exact [].
-  - simpl in H11; destruct H11.
-    exact ((existT _ a H11) :: (IHrules H12)).
+  - simpl in H; destruct H.
+    exact ((existT _ a H) :: (IHrules H0)).
 Defined.
 
 Lemma kc_nil : kind_consistent [] [].
@@ -383,13 +366,13 @@ Qed.
 Lemma kc_cons : forall init_regs regs r k v v', kind_consistent init_regs regs -> kind_consistent ((r,(existT _ k v)) :: init_regs) ((r, (existT _ k v')) :: regs).
 Proof.
   intros.
-  intros r' k'; split; intro; rewrite lookup_cons in *; destruct (r' =? r) eqn:G; destruct H12.
-  - inversion H12.
+  intros r' k'; split; intro; rewrite lookup_cons in *; destruct (r' =? r) eqn:G; destruct H0.
+  - inversion H0.
     eexists; auto.
-  - apply (kc_init_sim H11 _ H12).
-  - inversion H12.
+  - apply (kc_init_sim H _ H0).
+  - inversion H0.
     eexists; auto.
-  - apply (kc_sim_init H11 _ H12).
+  - apply (kc_sim_init H _ H0).
 Qed.
 
 Lemma init_regs_kc : forall init_regs, kind_consistent init_regs (initialize_SimRegs init_regs).
@@ -402,8 +385,8 @@ Proof.
     destruct r; apply kc_cons; auto.
 Qed.
 
-Definition eval_Basemodule_rr{E}`{Environment E}(env : E)(args : list (string * string))(rfbs : list RegFileBase)(timeout : nat)(meths : list (string * Signature))(basemod : BaseModule)(wf : WfBaseModule_new eval_K basemod) : mkProd (List.map dec_sig meths) -> M unit. refine (
-  match basemod return WfBaseModule_new eval_K basemod -> _ with
+Definition eval_Basemodule_rr{E}`{Environment E}(env : E)(args : list (string * string))(rfbs : list RegFileBase)(timeout : nat)(meths : list (string * Signature))(basemod : BaseModule)(wf : WfBaseModule_new eval_Kind basemod) : mkProd (List.map dec_sig meths) -> IO unit. refine (
+  match basemod return WfBaseModule_new eval_Kind basemod -> _ with
   | BaseRegFile rf => fun pf fs => _
   | BaseMod regs rules dms =>
       match rules with
@@ -416,36 +399,22 @@ Proof.
   - unfold WfBaseModule_new in pf.
     destruct pf.
     refine (do state <- initialize_files args rfbs;
-    eval_Rules env state (timeout * (List.length rules)) meths _ (unwind_list (get_wf_rules _ _ H12) _) fs).
+    eval_Rules env state (timeout * (List.length rules)) meths _ (unwind_list (get_wf_rules _ _ H0) _) fs).
     + apply init_regs_kc.
     + simpl.
-      destruct H12; discriminate.
+      destruct H0; discriminate.
 Defined.
 
-Definition eval_BaseMod{E}`{Environment E}(env : E)(args : list (string * string))(rfbs : list RegFileBase)(timeout : nat)(meths : list (string * Signature))(basemod : BaseModule)(wf : WfBaseModule_new eval_K basemod) :=
+Definition eval_BaseMod{E}`{Environment E}(env : E)(args : list (string * string))(rfbs : list RegFileBase)(timeout : nat)(meths : list (string * Signature))(basemod : BaseModule)(wf : WfBaseModule_new eval_Kind basemod) :=
   curry _ (eval_Basemodule_rr env args rfbs timeout meths wf).
 
 End Regs2.
 
 End EvalAction.
 
-Definition eval_BaseMod_Haskell := @eval_BaseMod HWord HVec HMap IO HArray _ _ _ _.
-
 Section Eval_Wf.
 
-Variable Word : nat -> Type.
-Variable Vec : nat -> Type -> Type.
-Variable Map : Type -> Type.
-Variable M : Type -> Type.
-Variable Arr : Type -> Type.
-
-Context `{IsWord Word}.
-Context `{IsVector Vec}.
-Context `{StringMap Map}.
-Context `{IOMonad Word Vec M}.
-Context `{IsArray Word Vec IO Arr}.
-
-Definition eval_BaseMod_Wf{E}`{Environment _ _ _ _ _ E}(env : E)(args : list (string * string))(rfbs : list RegFileBase)(timeout : nat)(meths : list (string * Signature))(basemod : BaseModule)(wf : WfBaseModule (eval_K Word Vec) basemod) :=
+Definition eval_BaseMod_Wf{E}`{Environment E}(env : E)(args : list (string * string))(rfbs : list RegFileBase)(timeout : nat)(meths : list (string * Signature))(basemod : BaseModule)(wf : WfBaseModule (eval_Kind) basemod) :=
   curry _ (eval_Basemodule_rr env args rfbs timeout meths (WfBaseModule_WfBaseModule_new wf)).
 
 End Eval_Wf.
