Simulator/CoqSim/HaskellTypes.v
@@ -1,51 +1,34 @@
-Require Import Kami.Simulator.CoqSim.SimTypes.
 Require Extraction.
-Require Import String.
+Require Import String Fin.
 
 Extraction Language Haskell.
 
-(* We postulate Haskell's more efficient datatypes and package them for extraction *)
+(* We postulate Haskell's more efficient datatypes and extract them *)
 
-(* Maps *)
+(* Maps with string keys *)
 
-Parameter HMap : Type -> Type.
+Parameter Map : Type -> Type.
 
-Parameter Hempty : forall {V}, HMap V.
-Parameter Hmap_lookup : forall {V}, string -> HMap V -> option V.
-Parameter Hinsert : forall {V}, string -> V -> HMap V -> HMap V.
+Parameter empty : forall {V}, Map V.
+Parameter map_lookup : forall {V}, string -> Map V -> option V.
+Parameter insert : forall {V}, string -> V -> Map V -> Map V.
 
-Instance HMapIsMap : StringMap HMap := {|
-  empty := @Hempty;
-  map_lookup := @Hmap_lookup;
-  insert := @Hinsert
-  |}.
-
-Extract Constant HMap "v" => "Data.Map.Map Prelude.String v".
-Extract Constant Hempty => "Data.Map.empty".
-Extract Constant Hmap_lookup => "Data.Map.lookup".
-Extract Constant Hinsert => "Data.Map.insert".
+Extract Constant Map "v" => "Data.Map.Map Prelude.String v".
+Extract Constant empty => "Data.Map.empty".
+Extract Constant map_lookup => "Data.Map.lookup".
+Extract Constant insert => "Data.Map.insert".
 
 (* Vectors *)
 
-Parameter HVec : nat -> Type -> Type.
+Parameter Vector : nat -> Type -> Type.
 
-Parameter Hindex : forall {X n}, Fin.t n -> HVec n X -> X.
-Parameter Hmap : forall {X Y n}, (X -> Y) -> HVec n X -> HVec n Y.
-Parameter Heq : forall {X n}, (X -> X -> bool) -> HVec n X -> HVec n X -> bool.
-Parameter Hto_list : forall {X n}, HVec n X -> list X.
-Parameter Hmake_vec : forall {X n}, (Fin.t n -> X) -> HVec n X.
-Parameter Hslice : forall {X n} (i m : nat),  HVec n X -> HVec m X.
-Parameter Hupdates : forall {X n}, HVec n X -> list (nat * X) -> HVec n X.
-
-Instance HVecIsVec : IsVector HVec := {|
-  SimTypes.index := @Hindex;
-  vec_map := @Hmap;
-  vec_eq := @Heq;
-  vec_to_list := @Hto_list;
-  make_vec := @Hmake_vec;
-  slice := @Hslice;
-  updates := @Hupdates
-  |}.
+Parameter vector_index : forall {X n}, Fin.t n -> Vector n X -> X.
+Parameter vector_map : forall {X Y n}, (X -> Y) -> Vector n X -> Vector n Y.
+Parameter vector_eq : forall {X n}, (X -> X -> bool) -> Vector n X -> Vector n X -> bool.
+Parameter vector_to_list : forall {X n}, Vector n X -> list X.
+Parameter make_vector : forall {X n}, (Fin.t n -> X) -> Vector n X.
+Parameter vector_slice : forall {X n} (i m : nat),  Vector n X -> Vector m X.
+Parameter vector_updates : forall {X n}, Vector n X -> list (nat * X) -> Vector n X.
 
 Fixpoint Fin_to_list{X n} : (Fin.t n -> X) -> list X :=
   match n with
@@ -53,149 +36,110 @@ Fixpoint Fin_to_list{X n} : (Fin.t n -> X) -> list X :=
   | S m => fun f => cons (f Fin.F1) (Fin_to_list (fun i => f (Fin.FS i)))
   end.
 
-Extract Constant HVec "a" => "Data.Vector.Vector a".
-Extract Constant Hindex => "(\_ (n,i) v -> v Data.Vector.! i)".
-Extract Constant Hmap => "(\_ -> Data.Vector.map)".
-Extract Constant Heq => "(\_ eqb v1 v2 -> Data.Vector.foldr (Prelude.&&) Prelude.True (Data.Vector.zipWith eqb v1 v2))".
-Extract Constant Hto_list => "(\ _ -> Data.Vector.toList)".
-Extract Constant Hmake_vec => "(\n f -> Data.Vector.fromList (coq_Fin_to_list n f))".
-Extract Constant Hslice => "(\_ i m v -> Data.Vector.slice i m v)".
-Extract Constant Hupdates => "(\_ -> (Data.Vector.//))".
+Extract Constant Vector "a" => "Data.Vector.Vector a".
+Extract Constant vector_index => "(\_ (n,i) v -> v Data.Vector.! i)".
+Extract Constant vector_map => "(\_ -> Data.Vector.map)".
+Extract Constant vector_eq => "(\_ eqb v1 v2 -> Data.Vector.foldr (Prelude.&&) Prelude.True (Data.Vector.zipWith eqb v1 v2))".
+Extract Constant vector_to_list => "(\ _ -> Data.Vector.toList)".
+Extract Constant make_vector => "(\n f -> Data.Vector.fromList (coq_Fin_to_list n f))".
+Extract Constant vector_slice => "(\_ i m v -> Data.Vector.slice i m v)".
+Extract Constant vector_updates => "(\_ -> (Data.Vector.//))".
 
-(* Words *)
+(* BVs *)
 
-Parameter HWord : nat -> Type.
-Parameter Hinv : forall {m}, HWord m -> HWord m.
-Parameter Htrunc_lsb : forall {m n}, HWord (m + n) -> HWord m.
-Parameter Htrunc_msb : forall {m n}, HWord (m + n) -> HWord n.
-Parameter Huand : forall {m}, HWord m -> HWord 1.
-Parameter Huor : forall {m}, HWord m -> HWord 1.
-Parameter Huxor : forall {m}, HWord m -> HWord 1.
-Parameter Hsub : forall {m}, HWord m -> HWord m -> HWord m.
-Parameter Hdiv : forall {m}, HWord m -> HWord m -> HWord m.
-Parameter Hrem : forall {m}, HWord m -> HWord m -> HWord m.
-Parameter Hsll : forall {m n}, HWord m -> HWord n -> HWord m.
-Parameter Hsrl : forall {m n}, HWord m -> HWord n -> HWord m.
-Parameter Hsra : forall {m n}, HWord m -> HWord n -> HWord m.
-Parameter Hconcat : forall {m n}, HWord m -> HWord n -> HWord (n + m).
-Parameter Hadd : forall {m}, list (HWord m) -> HWord m.
-Parameter Hmul : forall {m}, list (HWord m) -> HWord m.
-Parameter Hband : forall {m}, list (HWord m) -> HWord m.
-Parameter Hbor : forall {m}, list (HWord m) -> HWord m.
-Parameter Hbxor : forall {m}, list (HWord m) -> HWord m.
-Parameter Hwltb : forall {m}, HWord m -> HWord m -> bool.
-Parameter Hweqb : forall {m}, HWord m -> HWord m -> bool.
-Parameter Hword_to_nat : forall {m}, HWord m -> nat.
-Parameter Hnat_to_word : forall {m}, nat -> HWord m.
-Parameter Hprint_word_bin : forall {m}, HWord m -> string.
-Parameter Hprint_word_dec : forall {m}, HWord m -> string.
-Parameter Hprint_word_hex : forall {m}, HWord m -> string.
+Parameter BV : nat -> Type.
+Parameter bv_inv : forall {m}, BV m -> BV m.
+Parameter bv_trunc_lsb : forall {m n}, BV (m + n) -> BV m.
+Parameter bv_trunc_msb : forall {m n}, BV (m + n) -> BV n.
+Parameter bv_uand : forall {m}, BV m -> BV 1.
+Parameter bv_uor : forall {m}, BV m -> BV 1.
+Parameter bv_uxor : forall {m}, BV m -> BV 1.
+Parameter bv_sub : forall {m}, BV m -> BV m -> BV m.
+Parameter bv_div : forall {m}, BV m -> BV m -> BV m.
+Parameter bv_rem : forall {m}, BV m -> BV m -> BV m.
+Parameter bv_sll : forall {m n}, BV m -> BV n -> BV m.
+Parameter bv_srl : forall {m n}, BV m -> BV n -> BV m.
+Parameter bv_sra : forall {m n}, BV m -> BV n -> BV m.
+Parameter bv_concat : forall {m n}, BV m -> BV n -> BV (n + m).
+Parameter bv_add : forall {m}, list (BV m) -> BV m.
+Parameter bv_mul : forall {m}, list (BV m) -> BV m.
+Parameter bv_band : forall {m}, list (BV m) -> BV m.
+Parameter bv_bor : forall {m}, list (BV m) -> BV m.
+Parameter bv_bxor : forall {m}, list (BV m) -> BV m.
+Parameter bv_lt : forall {m}, BV m -> BV m -> bool.
+Parameter bv_eq : forall {m}, BV m -> BV m -> bool.
+Parameter bv_to_nat : forall {m}, BV m -> nat.
+Parameter nat_to_bv : forall {m}, nat -> BV m.
+Parameter print_bv_bin : forall {m}, BV m -> string.
+Parameter print_bv_dec : forall {m}, BV m -> string.
+Parameter print_bv_hex : forall {m}, BV m -> string.
 
-Instance HWordIsWord : IsWord HWord := {|
-  inv := @Hinv;
-  trunc_lsb := @Htrunc_lsb;
-  trunc_msb := @Htrunc_msb;
-  uand := @Huand;
-  uor := @Huor;
-  uxor := @Huxor;
-  sub := @Hsub;
-  div := @Hdiv;
-  rem := @Hrem;
-  sll := @Hsll;
-  srl := @Hsrl;
-  sra := @Hsra;
-  SimTypes.concat := @Hconcat;
-  add := @Hadd;
-  mul := @Hmul;
-  band := @Hband;
-  bor := @Hbor;
-  bxor := @Hbxor;
-  wltb := @Hwltb;
-  weqb := @Hweqb;
-  word_to_nat := @Hword_to_nat;
-  nat_to_word := @Hnat_to_word;
-  print_word_bin := @Hprint_word_bin;
-  print_word_dec := @Hprint_word_dec;
-  print_word_hex := @Hprint_word_hex
-  |}.
-
-Extract Constant HWord => "Data.BitVector.BV".
-Extract Constant Hinv => "(\_ -> Data.BitVector.not)".
-Extract Constant Htrunc_lsb => "(\m _ -> if m Prelude.== 0 then Prelude.const Data.BitVector.nil else Data.BitVector.least m)".
-Extract Constant Htrunc_msb => "(\_ n -> if n Prelude.== 0 then Prelude.const Data.BitVector.nil else Data.BitVector.most n)".
-Extract Constant Huand => "(\_ v -> Data.BitVector.fromBool (Data.BitVector.foldr (Prelude.&&) Prelude.True v))".
-Extract Constant Huor => "(\_ v -> Data.BitVector.fromBool (Data.BitVector.foldr (Prelude.||) Prelude.False v))".
-Extract Constant Huxor => "(\_ v -> Data.BitVector.fromBool (Data.BitVector.foldr (Prelude./=) Prelude.False v))".
-Extract Constant Hsub => "(\_ -> (Prelude.-))".
-Extract Constant Hdiv => "(\_ -> Prelude.div)".
-Extract Constant Hrem => "(\_ -> Prelude.rem)".
-Extract Constant Hsll => "(\_ _ -> Data.BitVector.shl)".
-Extract Constant Hsrl => "(\_ _ -> Data.BitVector.shr)".
-Extract Constant Hsra => "(\_ _ -> Data.BitVector.ashr)".
-Extract Constant Hconcat => "(\_ _ -> (Data.BitVector.#))".
-Extract Constant Hadd => "(\_ -> Prelude.foldr (Prelude.+) 0)".
-Extract Constant Hmul => "(\_ -> Prelude.foldr (Prelude.*) 1)".
-Extract Constant Hband => "(\n -> Prelude.foldr (Data.Bits..&.) (Data.BitVector.ones n))".
-Extract Constant Hbor => "(\n -> Prelude.foldr (Data.Bits..|.) (Data.BitVector.zeros n))".
-Extract Constant Hbxor => "(\n -> Prelude.foldr Data.Bits.xor (Data.BitVector.zeros n))".
-Extract Constant Hwltb => "(\_ -> (Data.BitVector.<.))".
-Extract Constant Hweqb => "(\_ -> (Data.BitVector.==.))".
-Extract Constant Hword_to_nat => "(\_ x -> Prelude.fromIntegral (Data.BitVector.nat x))".
-Extract Inlined Constant Hnat_to_word => "Data.BitVector.bitVec".
-Extract Constant Hprint_word_bin => "(\_ -> CustomExtract.bv_bin)".
-Extract Constant Hprint_word_dec => "(\_ -> CustomExtract.bv_dec)".
-Extract Constant Hprint_word_hex => "(\_ -> CustomExtract.bv_hex)".
+Extract Constant BV => "Data.BitVector.BV".
+Extract Constant bv_inv => "(\_ -> Data.BitVector.not)".
+Extract Constant bv_trunc_lsb => "(\m _ -> if m Prelude.== 0 then Prelude.const Data.BitVector.nil else Data.BitVector.least m)".
+Extract Constant bv_trunc_msb => "(\_ n -> if n Prelude.== 0 then Prelude.const Data.BitVector.nil else Data.BitVector.most n)".
+Extract Constant bv_uand => "(\_ v -> Data.BitVector.fromBool (Data.BitVector.foldr (Prelude.&&) Prelude.True v))".
+Extract Constant bv_uor => "(\_ v -> Data.BitVector.fromBool (Data.BitVector.foldr (Prelude.||) Prelude.False v))".
+Extract Constant bv_uxor => "(\_ v -> Data.BitVector.fromBool (Data.BitVector.foldr (Prelude./=) Prelude.False v))".
+Extract Constant bv_sub => "(\_ -> (Prelude.-))".
+Extract Constant bv_div => "(\_ -> Prelude.div)".
+Extract Constant bv_rem => "(\_ -> Prelude.rem)".
+Extract Constant bv_sll => "(\_ _ -> Data.BitVector.shl)".
+Extract Constant bv_srl => "(\_ _ -> Data.BitVector.shr)".
+Extract Constant bv_sra => "(\_ _ -> Data.BitVector.ashr)".
+Extract Constant bv_concat => "(\_ _ -> (Data.BitVector.#))".
+Extract Constant bv_add => "(\_ -> Prelude.foldr (Prelude.+) 0)".
+Extract Constant bv_mul => "(\_ -> Prelude.foldr (Prelude.*) 1)".
+Extract Constant bv_band => "(\n -> Prelude.foldr (Data.Bits..&.) (Data.BitVector.ones n))".
+Extract Constant bv_bor => "(\n -> Prelude.foldr (Data.Bits..|.) (Data.BitVector.zeros n))".
+Extract Constant bv_bxor => "(\n -> Prelude.foldr Data.Bits.xor (Data.BitVector.zeros n))".
+Extract Constant bv_lt => "(\_ -> (Data.BitVector.<.))".
+Extract Constant bv_eq => "(\_ -> (Data.BitVector.==.))".
+Extract Constant bv_to_nat => "(\_ x -> Prelude.fromIntegral (Data.BitVector.nat x))".
+Extract Inlined Constant nat_to_bv => "Data.BitVector.bitVec".
+Extract Constant print_bv_bin => "(\_ -> CustomExtract.bv_bin)".
+Extract Constant print_bv_dec => "(\_ -> CustomExtract.bv_dec)".
+Extract Constant print_bv_hex => "(\_ -> CustomExtract.bv_hex)".
 
 (* IO *)
 
 Require Import String.
 
 Parameter IO : Type -> Type.
-Parameter Hret : forall {X}, X -> IO X.
-Parameter Hbind : forall {X Y}, IO X -> (X -> IO Y) -> IO Y.
-Parameter Herror : forall {X}, string -> IO X.
-Parameter Hprint : string -> IO unit.
-Parameter Hrand_bool : IO bool.
-Parameter Hrand_word : forall n, IO (HWord n).
-Parameter Hrand_vec : forall {X n}, IO X -> IO (HVec n X).
-Parameter Hexit : forall {X}, IO X.
-
-Instance IOPrintMonad : IOMonad IO := {|
-  ret := @Hret;
-  bind := @Hbind;
-  error := @Herror;
-  print := Hprint;
-  rand_bool := Hrand_bool;
-  rand_word := Hrand_word;
-  rand_vec := @Hrand_vec;
-  exit := @Hexit
-  |}.
+Parameter ret : forall {X}, X -> IO X.
+Parameter bind : forall {X Y}, IO X -> (X -> IO Y) -> IO Y.
+Parameter error : forall {X}, string -> IO X.
+Parameter print : string -> IO unit.
+Parameter rand_bool : IO bool.
+Parameter rand_bv : forall n, IO (BV n).
+Parameter rand_vector : forall {X n}, IO X -> IO (Vector n X).
+Parameter exit : forall {X}, IO X.
 
 Extract Constant IO "a" => "Prelude.IO a".
-Extract Inlined Constant Hret => "Prelude.return".
-Extract Inlined Constant Hbind => "(GHC.Base.>>=)".
-Extract Inlined Constant Herror => "Prelude.error".
+Extract Inlined Constant ret => "Prelude.return".
+Extract Inlined Constant bind => "(GHC.Base.>>=)".
+Extract Inlined Constant error => "Prelude.error".
 (*Extract Constant Hprint => "(\str -> (GHC.Base.>>) (Prelude.putStrLn str) (System.IO.hFlush System.IO.stdout))". *)
-Extract Inlined Constant Hprint => "Prelude.putStr".
-Extract Constant Hrand_bool => "Prelude.return Prelude.False". (*FIXME*)
-Extract Constant Hrand_word => "Prelude.undefined". (*FIXME*)
-Extract Constant Hrand_vec => "Prelude.undefined". (*FIXME*)
-Extract Constant Hexit => "System.Exit.exitSuccess".
+Extract Inlined Constant print => "Prelude.putStr".
+Extract Constant rand_bool => "Prelude.return Prelude.False". (*FIXME*)
+Extract Constant rand_bv => "Prelude.undefined". (*FIXME*)
+Extract Constant rand_vector => "Prelude.undefined". (*FIXME*)
+Extract Constant exit => "System.Exit.exitSuccess".
+
+Module Notations.
+
+Notation "'do' x <- y ; cont" := (bind y (fun x => cont)) (at level 20).
+
+End Notations.
 
 (* Arrays *)
 
-Parameter HArray : Type -> Type.
-Parameter Harr_repl : forall {X}, nat -> X -> IO (HArray X).
-Parameter Harr_slice : forall {X} (i m : nat), HArray X -> IO (HVec m X).
-Parameter Harr_updates : forall {X}, HArray X -> list (nat * X) -> IO unit.
-Parameter Harr_new : forall {X}, nat -> IO (HArray X).
-
-Instance HArrayIsArray : IsArray HArray := {|
-  arr_repl := @Harr_repl;
-  arr_slice := @Harr_slice;
-  arr_updates := @Harr_updates
-  |}.
-
+Parameter Arr : Type -> Type.
+Parameter arr_repl : forall {X}, nat -> X -> IO (Arr X).
+Parameter arr_slice : forall {X} (i m : nat), Arr X -> IO (Vector m X).
+Parameter arr_updates : forall {X}, Arr X -> list (nat * X) -> IO unit.
+(* Parameter arr_new : forall {X}, nat -> IO (Array X).
+ *)
 (** does not work at the moment **)
 (*Extract Constant HArray "a" => "Data.Array.IO.IOArray Prelude.Int a".
 Extract Constant Harr_repl => "(\n x -> Data.Array.MArray.newArray (0, n Prelude.- 1) x)".
@@ -203,7 +147,7 @@ Extract Constant Harr_slice => "(\i m a -> Control.Monad.liftM Data.Vector.fromL
 Extract Constant Harr_updates => "(\a ps -> Control.Monad.foldM (\_ (i,e) -> Data.Array.MArray.writeArray a i e) () ps)".*)
 
 
-Extract Constant HArray "a" => "Data.Vector.Mutable.MVector (Control.Monad.Primitive.PrimState Prelude.IO) a".
-Extract Constant Harr_repl => "Data.Vector.Mutable.replicate".
-Extract Constant Harr_slice => "(\i m a -> Data.Vector.Generic.freeze (Data.Vector.Mutable.slice i m a))".
-Extract Constant Harr_updates => "(\a ps -> Control.Monad.foldM (\_ (i,x) -> Data.Vector.Mutable.write a i x) () ps)".
+Extract Constant Arr "a" => "Data.Vector.Mutable.MVector (Control.Monad.Primitive.PrimState Prelude.IO) a".
+Extract Constant arr_repl => "Data.Vector.Mutable.replicate".
+Extract Constant arr_slice => "(\i m a -> Data.Vector.Generic.freeze (Data.Vector.Mutable.slice i m a))".
+Extract Constant arr_updates => "(\a ps -> Control.Monad.foldM (\_ (i,x) -> Data.Vector.Mutable.write a i x) () ps)".
